Added a get_key function to the heaps
This is a bit more realistic, in the the heap elements don't have to be
linearly ordered, only their keys do.

examples/miniML/okasaki-examples/SplayHeapScript.sml
@@ -9,11 +9,10 @@ val cases_on = Cases_on;
 val every_case_tac = BasicProvers.EVERY_CASE_TAC;
 val full_case_tac = BasicProvers.FULL_CASE_TAC;
 
-
 val _ = new_theory "SplayHeap"
 
 val _ = Hol_datatype `
-heaps = Empty | Node of heaps => 'a => heaps`;
+heap = Empty | Node of heap => 'a => heap`;
 
 val splay_heap_to_bag_def = Define `
 (splay_heap_to_bag Empty = {||}) ∧
@@ -21,12 +20,12 @@ val splay_heap_to_bag_def = Define `
   BAG_INSERT x (BAG_UNION (splay_heap_to_bag h1) (splay_heap_to_bag h2)))`;
 
 val splay_heap_ok_def = Define `
-(splay_heap_ok leq Empty = T) ∧
-(splay_heap_ok leq (Node h1 x h2) =
-  splay_heap_ok leq h1 ∧
-  splay_heap_ok leq h2 ∧
-  BAG_EVERY (\y. leq y x) (splay_heap_to_bag h1) ∧
-  BAG_EVERY (\y. leq x y) (splay_heap_to_bag h2))`;
+(splay_heap_ok get_key leq Empty = T) ∧
+(splay_heap_ok get_key leq (Node h1 x h2) =
+  splay_heap_ok get_key leq h1 ∧
+  splay_heap_ok get_key leq h2 ∧
+  BAG_EVERY (\y. leq (get_key y) (get_key x)) (splay_heap_to_bag h1) ∧
+  BAG_EVERY (\y. leq (get_key x) (get_key y)) (splay_heap_to_bag h2))`;
 
 val _ = Define `
 empty = Empty`;
@@ -36,52 +35,52 @@ val _ = Define `
 (is_empty _ = F)`;
 
 val partition_def = Define `
-(partition leq pivot Empty = (Empty, Empty)) ∧
-(partition leq pivot (Node a x b) =
-  if leq x pivot then
+(partition get_key leq pivot Empty = (Empty, Empty)) ∧
+(partition get_key leq pivot (Node a x b) =
+  if leq (get_key x) (get_key pivot) then
     (case b of
         Empty => (Node a x b, Empty)
       | Node b1 y b2 =>
-          if leq y pivot then
-            let (small, big) = partition leq pivot b2 in
+          if leq (get_key y) (get_key pivot) then
+            let (small, big) = partition get_key leq pivot b2 in
               (Node (Node a x b1) y small, big)
           else
-            let (small, big) = partition leq pivot b1 in
+            let (small, big) = partition get_key leq pivot b1 in
               (Node a x small, Node big y b2))
   else
     (case a of
         Empty => (Empty, Node a x b)
       | Node a1 y a2 =>
-          if leq y pivot then
-            let (small, big) = partition leq pivot a2 in
+          if leq (get_key y) (get_key pivot) then
+            let (small, big) = partition get_key leq pivot a2 in
               (Node a1 y small, Node big x b)
           else
-            let (small, big) = partition leq pivot a1 in
+            let (small, big) = partition get_key leq pivot a1 in
               (small, Node big y (Node a2 x b))))`;
 
 val partition_ind = fetch "-" "partition_ind"
-val heaps_size_def = fetch "-" "heaps_size_def"
+val heap_size_def = fetch "-" "heap_size_def"
 
 val partition_size = Q.prove (
-`!leq p h1 h2 h3.
-  ((h2,h3) = partition leq p h1)
+`!get_key leq p h1 h2 h3.
+  ((h2,h3) = partition get_key leq p h1)
   ⇒
-  heaps_size f h2 ≤ heaps_size f h1 ∧
-  heaps_size f h3 ≤ heaps_size f h1`,
+  heap_size f h2 ≤ heap_size f h1 ∧
+  heap_size f h3 ≤ heap_size f h1`,
 recInduct partition_ind >>
-rw [heaps_size_def, partition_def] >>
+rw [heap_size_def, partition_def] >>
 every_case_tac >>
 fs [] >>
-rw [heaps_size_def] >>
-cases_on `partition leq pivot h0` >>
-cases_on `partition leq pivot h` >>
+rw [heap_size_def] >>
+cases_on `partition get_key leq pivot h0` >>
+cases_on `partition get_key leq pivot h` >>
 fs [LET_THM] >>
-rw [heaps_size_def] >>
+rw [heap_size_def] >>
 decide_tac);
 
 val partition_bags = Q.prove (
-`!leq p h1 h2 h3.
-  ((h2,h3) = partition leq p h1)
+`!get_key leq p h1 h2 h3.
+  ((h2,h3) = partition get_key leq p h1)
   ⇒
   (splay_heap_to_bag h1 =
    BAG_UNION (splay_heap_to_bag h2) (splay_heap_to_bag h3))`,
@@ -90,37 +89,37 @@ rw [partition_def, splay_heap_to_bag_def] >>
 every_case_tac >>
 fs [] >>
 rw [splay_heap_to_bag_def] >>
-cases_on `partition leq pivot h0` >>
-cases_on `partition leq pivot h` >>
+cases_on `partition get_key leq pivot h0` >>
+cases_on `partition get_key leq pivot h` >>
 fs [LET_THM] >>
 rw [splay_heap_to_bag_def, BAG_UNION_INSERT] >>
 metis_tac [ASSOC_BAG_UNION, COMM_BAG_UNION, BAG_INSERT_commutes]);
 
 val partition_split = Q.prove (
-`!leq p h1 h2 h3.
+`!get_key leq p h1 h2 h3.
   transitive leq ∧
   trichotomous leq ∧
-  ((h2,h3) = partition leq p h1) ∧
-  splay_heap_ok leq h1
+  ((h2,h3) = partition get_key leq p h1) ∧
+  splay_heap_ok get_key leq h1
   ⇒
-  BAG_EVERY (\y. leq y p) (splay_heap_to_bag h2) ∧
-  BAG_EVERY (\y. ¬leq y p) (splay_heap_to_bag h3)`,
+  BAG_EVERY (\y. leq (get_key y) (get_key p)) (splay_heap_to_bag h2) ∧
+  BAG_EVERY (\y. ¬leq (get_key y) (get_key p)) (splay_heap_to_bag h3)`,
 recInduct partition_ind >>
 rw [partition_def, splay_heap_to_bag_def, splay_heap_ok_def] >>
 every_case_tac >>
 fs [] >>
 rw [] >>
 fs [splay_heap_ok_def, splay_heap_to_bag_def] >>
-cases_on `partition leq pivot h0` >>
-cases_on `partition leq pivot h` >>
+cases_on `partition get_key leq pivot h0` >>
+cases_on `partition get_key leq pivot h` >>
 fs [LET_THM, splay_heap_to_bag_def] >>
 rw [] >>
 fs [BAG_EVERY, transitive_def, trichotomous] >>
 metis_tac []);
 
 val partition_ok_lem = Q.prove (
-`!leq p h1 h2 h3.
-  (partition leq p h1 = (h2, h3)) ⇒
+`!get_key leq p h1 h2 h3.
+  (partition get_key leq p h1 = (h2, h3)) ⇒
   BAG_EVERY P (splay_heap_to_bag h1) ⇒
   BAG_EVERY P (splay_heap_to_bag h2) ∧
   BAG_EVERY P (splay_heap_to_bag h3)`,
@@ -133,22 +132,22 @@ fs [] >>
 rw []);
 
 val partition_ok = Q.prove (
-`!leq p h1 h2 h3.
+`!get_key leq p h1 h2 h3.
   WeakLinearOrder leq ∧
-  ((h2,h3) = partition leq p h1) ∧
-  splay_heap_ok leq h1
+  ((h2,h3) = partition get_key leq p h1) ∧
+  splay_heap_ok get_key leq h1
   ⇒
-  splay_heap_ok leq h2 ∧
-  splay_heap_ok leq h3`,
+  splay_heap_ok get_key leq h2 ∧
+  splay_heap_ok get_key leq h3`,
 recInduct partition_ind >>
 RW_TAC pure_ss [] >>
-cases_on `leq x pivot` >>
+cases_on `leq (get_key x) (get_key pivot)` >>
 fs [partition_def, splay_heap_ok_def] >>
 every_case_tac >>
 fs [] >>
 rw [] >>
-cases_on `partition leq pivot h0` >>
-cases_on `partition leq pivot h` >>
+cases_on `partition get_key leq pivot h0` >>
+cases_on `partition get_key leq pivot h` >>
 fs [LET_THM, splay_heap_ok_def, splay_heap_to_bag_def] >>
 rw [] >-
 (fs [BAG_EVERY] >>
@@ -163,18 +162,18 @@ metis_tac [partition_ok_lem] >-
  metis_tac [transitive_def, WeakLinearOrder, WeakOrder]));
 
 val insert_def = Define `
-insert leq x t =
-  let (a, b) = partition leq x t in
+insert get_key leq x t =
+  let (a, b) = partition get_key leq x t in
     Node a x b`;
 
 val merge_def = tDefine "merge" `
-(merge leq Empty h2 = h2) ∧
-(merge leq (Node a x b) h2 =
-  let (ta, tb) = partition leq x h2 in
-    Node (merge leq ta a) x (merge leq tb b))`
-(WF_REL_TAC `measure (\(x,y,z).
-                        heaps_size (\_.1) y +
-                        heaps_size (\_.1) z)` >>
+(merge get_key leq Empty h2 = h2) ∧
+(merge get_key leq (Node a x b) h2 =
+  let (ta, tb) = partition get_key leq x h2 in
+    Node (merge get_key leq ta a) x (merge get_key leq tb b))`
+(WF_REL_TAC `measure (\(_,x,y,z).
+                        heap_size (\_.1) y +
+                        heap_size (\_.1) z)` >>
  rw [] >>
  imp_res_tac partition_size >>
  pop_assum (MP_TAC o Q.SPEC `(λ_.1)`) >>
@@ -197,8 +196,8 @@ val delete_min_def = Define `
 val delete_min_ind = fetch "-" "delete_min_ind"
 
 val splay_heap_insert_bag = Q.store_thm ("splay_heap_insert_bag",
-`!h leq x.
-  splay_heap_to_bag (insert leq x h) =
+`!h get_key leq x.
+  splay_heap_to_bag (insert get_key leq x h) =
   BAG_INSERT x (splay_heap_to_bag h)`,
 induct_on `h` >>
 rw [splay_heap_to_bag_def, insert_def] >>
@@ -208,88 +207,67 @@ imp_res_tac (GSYM partition_bags) >>
 fs [splay_heap_to_bag_def]);
 
 val splay_heap_insert_ok = Q.store_thm ("splay_heap_insert_ok",
-`!leq x h.
-  WeakLinearOrder leq ∧ splay_heap_ok leq h
+`!get_key leq x h.
+  WeakLinearOrder leq ∧ splay_heap_ok get_key leq h
   ⇒
-  splay_heap_ok leq (insert leq x h)`,
+  splay_heap_ok get_key leq (insert get_key leq x h)`,
 rw [insert_def, splay_heap_ok_def] >>
 rw [splay_heap_ok_def] >-
 metis_tac [partition_ok] >-
 metis_tac [partition_ok] >-
 metis_tac [WeakLinearOrder, WeakOrder, partition_split] >-
-(`BAG_EVERY (\y. ¬leq y x) (splay_heap_to_bag b)`
+(`BAG_EVERY (\y. ¬leq (get_key y) (get_key x)) (splay_heap_to_bag b)`
            by metis_tac [partition_split, WeakLinearOrder, WeakOrder] >>
  fs [BAG_EVERY] >>
  metis_tac [WeakLinearOrder_neg]));
 
 val splay_heap_merge_bag = Q.store_thm ("splay_heap_merge_bag",
-`!leq h1 h2.
-  (splay_heap_to_bag (merge leq h1 h2) =
+`!get_key leq h1 h2.
+  (splay_heap_to_bag (merge get_key leq h1 h2) =
     BAG_UNION (splay_heap_to_bag h1) (splay_heap_to_bag h2))`,
 recInduct merge_ind >>
 rw [merge_def, splay_heap_to_bag_def] >>
-cases_on `partition leq x h2` >>
+cases_on `partition get_key leq x h2` >>
 fs [] >>
 imp_res_tac (GSYM partition_bags) >>
 rw [splay_heap_to_bag_def, BAG_UNION_INSERT] >>
 metis_tac [ASSOC_BAG_UNION, COMM_BAG_UNION, BAG_INSERT_commutes]);
 
 val splay_heap_merge_ok = Q.store_thm ("splay_heap_merge_ok",
-`!leq h1 h2.
-  WeakLinearOrder leq ∧ splay_heap_ok leq h1 ∧ splay_heap_ok leq h2
+`!get_key leq h1 h2.
+  WeakLinearOrder leq ∧ splay_heap_ok get_key leq h1 ∧ splay_heap_ok get_key leq h2
   ⇒
-  splay_heap_ok leq (merge leq h1 h2)`,
+  splay_heap_ok get_key leq (merge get_key leq h1 h2)`,
 recInduct merge_ind >>
 rw [merge_def, splay_heap_ok_def] >>
 rw [splay_heap_ok_def, splay_heap_merge_bag] >-
 metis_tac [partition_ok] >-
 metis_tac [partition_ok] >-
 metis_tac [partition_split, WeakLinearOrder, WeakOrder] >-
-(`BAG_EVERY (\y. ¬leq y x) (splay_heap_to_bag tb)`
+(`BAG_EVERY (\y. ¬leq (get_key y) (get_key x)) (splay_heap_to_bag tb)`
            by metis_tac [partition_split, WeakLinearOrder, WeakOrder] >>
  fs [BAG_EVERY] >>
  metis_tac [WeakLinearOrder_neg]));
 
-val splay_heap_find_min = Q.prove (
-`!h x leq. WeakLinearOrder leq ∧ (h ≠ Empty) ∧ splay_heap_ok leq h ⇒
-  ((find_min h = x) =
-   (BAG_IN x (splay_heap_to_bag h) ∧
-    (!y. BAG_IN y (splay_heap_to_bag h) ⇒ leq x y)))`,
-recInduct find_min_ind >>
-rw [splay_heap_to_bag_def, splay_heap_ok_def, find_min_def] >-
-metis_tac [BAG_EVERY, WeakLinearOrder_neg, WeakLinearOrder, WeakOrder,
-           reflexive_def] >>
-EQ_TAC >>
-rw [] >-
-metis_tac [] >-
-(fs [BAG_EVERY] >>
- metis_tac [WeakLinearOrder, WeakOrder, transitive_def]) >-
-metis_tac [] >-
-metis_tac [] >-
-metis_tac [] >-
-(fs [BAG_EVERY] >>
- metis_tac [WeakLinearOrder, WeakOrder, transitive_def]) >-
-metis_tac [BAG_EVERY, WeakLinearOrder_neg, WeakLinearOrder, WeakOrder,
-           reflexive_def] >-
-metis_tac [] >-
-metis_tac [] >-
-metis_tac [] >-
-metis_tac [BAG_EVERY, WeakLinearOrder_neg, WeakLinearOrder, WeakOrder,
-           reflexive_def]);
-
 val splay_heap_find_min_thm = Q.store_thm ("splay_heap_find_min_thm",
-`!h leq. WeakLinearOrder leq ∧ (h ≠ Empty) ∧ splay_heap_ok leq h ⇒
+`!h get_key leq. 
+  WeakLinearOrder leq ∧ (h ≠ Empty) ∧ splay_heap_ok get_key leq h 
+  ⇒
   BAG_IN (find_min h) (splay_heap_to_bag h) ∧
-  (!y. BAG_IN y (splay_heap_to_bag h) ⇒ leq (find_min h) y)`,
-metis_tac [splay_heap_find_min]);
+  (!y. BAG_IN y (splay_heap_to_bag h) ⇒ 
+       leq (get_key (find_min h)) (get_key y))`,
+recInduct find_min_ind >>
+rw [splay_heap_to_bag_def, find_min_def] >>
+fs [splay_heap_ok_def, splay_heap_to_bag_def, BAG_EVERY] >> 
+metis_tac [WeakLinearOrder, WeakOrder, transitive_def, reflexive_def]);
 
 val splay_heap_delete_min_thm = Q.store_thm ("splay_heap_delete_min_thm",
-`!h leq.
+`!h get_key leq.
   WeakLinearOrder leq ∧
   (h ≠ Empty) ∧
-  splay_heap_ok leq h
+  splay_heap_ok get_key leq h
   ⇒
-  splay_heap_ok leq (delete_min h) ∧
+  splay_heap_ok get_key leq (delete_min h) ∧
   (splay_heap_to_bag (delete_min h) =
    BAG_DIFF (splay_heap_to_bag h) (EL_BAG (find_min h)))`,
 HO_MATCH_MP_TAC delete_min_ind >>
@@ -306,9 +284,9 @@ srw_tac [bagLib.BAG_ss]
      metis_tac [WeakLinearOrder, WeakOrder, transitive_def],
  res_tac >>
      srw_tac [BAG_AC_ss] [] >>
-     `splay_heap_ok leq (Node v6 v7 v8)` by rw [splay_heap_ok_def] >>
+     `splay_heap_ok get_key leq (Node v6 v7 v8)` by rw [splay_heap_ok_def] >>
      `BAG_IN (find_min (Node v6 v7 v8)) (splay_heap_to_bag (Node v6 v7 v8))`
-          by metis_tac [splay_heap_find_min_thm, fetch "-" "heaps_distinct"] >>
+          by metis_tac [splay_heap_find_min_thm, fetch "-" "heap_distinct"] >>
      fs [splay_heap_to_bag_def] >>
      `SUB_BAG (EL_BAG (find_min (Node v6 v7 v8)))
               (EL_BAG v7 ⊎ (splay_heap_to_bag v6 ⊎ splay_heap_to_bag v8))`
