examples/miniML/okasaki-examples/PairingHeapScript.sml
@@ -24,11 +24,11 @@ val pairing_heap_to_bag_def = Define `
   BAG_UNION (pairing_heap_to_bag h) (pairing_heaps_to_bag hs))`;
 
 val pairing_heap_ok_def = tDefine "pairing_heap_ok" `
-(pairing_heap_ok leq Empty = T) ∧
-(pairing_heap_ok leq (Node x hs) = 
-  EVERY (pairing_heap_ok leq) hs ∧
-  BAG_EVERY (\y. leq x y) (pairing_heaps_to_bag hs))`
-(wf_rel_tac `measure (\(_,h). (heap_size (\x.1) h))` >>
+(pairing_heap_ok get_key leq Empty = T) ∧
+(pairing_heap_ok get_key leq (Node x hs) = 
+  EVERY (pairing_heap_ok get_key leq) hs ∧
+  BAG_EVERY (\y. leq (get_key x) (get_key y)) (pairing_heaps_to_bag hs))`
+(wf_rel_tac `measure (\(_,_,h). (heap_size (\x.1) h))` >>
 rw [] >>
 induct_on `hs` >>
 rw [fetch "-" "heap_size_def"] >>
@@ -43,10 +43,10 @@ val is_empty = Define `
 (is_empty _ = F)`;
 
 val merge_def = Define `
-(merge leq h Empty = h) ∧
-(merge leq Empty h = h) ∧
-(merge leq (Node x hs1) (Node y hs2) =
-  if leq x y then
+(merge get_key leq h Empty = h) ∧
+(merge get_key leq Empty h = h) ∧
+(merge get_key leq (Node x hs1) (Node y hs2) =
+  if leq (get_key x) (get_key y) then
     Node x (Node y hs2 :: hs1)
   else 
     Node y (Node x hs1 :: hs2))`;
@@ -54,13 +54,13 @@ val merge_def = Define `
 val merge_ind = fetch "-" "merge_ind"
 
 val insert_def = Define `
-insert leq x h = merge leq (Node x []) h`;
+insert get_key leq x h = merge get_key leq (Node x []) h`;
 
 val merge_pairs_def = Define `
-(merge_pairs leq [] = Empty) ∧
-(merge_pairs leq [h] = h) ∧
-(merge_pairs leq (h1::h2::hs) = 
-  merge leq (merge leq h1 h2) (merge_pairs leq hs))`;
+(merge_pairs get_key leq [] = Empty) ∧
+(merge_pairs get_key leq [h] = h) ∧
+(merge_pairs get_key leq (h1::h2::hs) = 
+  merge get_key leq (merge get_key leq h1 h2) (merge_pairs get_key leq hs))`;
 
 val merge_pairs_ind = fetch "-" "merge_pairs_ind"
 
@@ -68,46 +68,49 @@ val find_min_def = Define `
 find_min (Node x _) = x`;
 
 val delete_min_def = Define `
-delete_min leq (Node x hs) = merge_pairs leq hs`;
+delete_min get_key leq (Node x hs) = merge_pairs get_key leq hs`;
 
 val pairing_heap_merge_bag = Q.store_thm ("pairing_heap_merge_bag",
-`!leq h1 h2.
-  pairing_heap_to_bag (merge leq h1 h2) = 
+`!get_key leq h1 h2.
+  pairing_heap_to_bag (merge get_key leq h1 h2) = 
   BAG_UNION (pairing_heap_to_bag h1) (pairing_heap_to_bag h2)`,
 HO_MATCH_MP_TAC merge_ind >>
 srw_tac [BAG_AC_ss] [merge_def, pairing_heap_to_bag_def, BAG_INSERT_UNION]);
 
 val pairing_heap_merge_ok = Q.store_thm ("pairing_heap_merge_ok",
-`!leq h1 h2. 
-  WeakLinearOrder leq ∧ pairing_heap_ok leq h1 ∧ pairing_heap_ok leq h2 
+`!get_key leq h1 h2. 
+  WeakLinearOrder leq ∧ 
+  pairing_heap_ok get_key leq h1 ∧ 
+  pairing_heap_ok get_key leq h2 
   ⇒ 
-  pairing_heap_ok leq (merge leq h1 h2)`,
+  pairing_heap_ok get_key leq (merge get_key leq h1 h2)`,
 HO_MATCH_MP_TAC merge_ind >>
 rw [merge_def, pairing_heap_ok_def, pairing_heap_to_bag_def] >>
-metis_tac [BAG_EVERY, WeakLinearOrder, WeakOrder, transitive_def,
-           WeakLinearOrder_neg]);
+fs [BAG_EVERY] >>
+metis_tac [WeakLinearOrder, WeakOrder, transitive_def, WeakLinearOrder_neg]);
 
 val pairing_heap_insert_bag = Q.store_thm ("pairing_heap_insert_bag",
-`!h leq x.
-  pairing_heap_to_bag (insert leq x h) =
+`!h get_key leq x.
+  pairing_heap_to_bag (insert get_key leq x h) =
   BAG_INSERT x (pairing_heap_to_bag h)`,
 rw [insert_def, pairing_heap_merge_bag, pairing_heap_to_bag_def,
     BAG_INSERT_UNION]);
 
 val pairing_heap_insert_ok = Q.store_thm ("pairing_heap_insert_ok",
-`!leq x h. 
-  WeakLinearOrder leq ∧ pairing_heap_ok leq h 
+`!get_key leq x h. 
+  WeakLinearOrder leq ∧ pairing_heap_ok get_key leq h 
   ⇒ 
-  pairing_heap_ok leq (insert leq x h)`,
+  pairing_heap_ok get_key leq (insert get_key leq x h)`,
 rw [insert_def] >>
-`pairing_heap_ok leq (Node x [])` 
+`pairing_heap_ok get_key leq (Node x [])` 
          by rw [pairing_heap_ok_def, pairing_heap_to_bag_def] >>
 metis_tac [pairing_heap_merge_ok]);
 
 val pairing_heap_find_min_thm = Q.store_thm ("pairing_heap_find_min_thm",
-`!h leq. WeakLinearOrder leq ∧ (h ≠ Empty) ∧ pairing_heap_ok leq h ⇒
+`!h get_key leq. WeakLinearOrder leq ∧ (h ≠ Empty) ∧ pairing_heap_ok get_key leq h ⇒
   BAG_IN (find_min h) (pairing_heap_to_bag h) ∧
-  (!y. BAG_IN y (pairing_heap_to_bag h) ⇒ leq (find_min h) y)`,
+  (!y. BAG_IN y (pairing_heap_to_bag h) ⇒ 
+       leq (get_key (find_min h)) (get_key y))`,
 rw [] >>
 cases_on `h` >>
 fs [find_min_def, pairing_heap_to_bag_def, pairing_heap_ok_def] >>
@@ -115,27 +118,27 @@ fs [BAG_EVERY] >>
 metis_tac [WeakLinearOrder, WeakOrder, reflexive_def]);
 
 val pairing_heap_merge_pairs_bag = Q.prove (
-`!leq hs. pairing_heap_to_bag (merge_pairs leq hs) = pairing_heaps_to_bag hs`,
+`!get_key leq hs. pairing_heap_to_bag (merge_pairs get_key leq hs) = pairing_heaps_to_bag hs`,
 recInduct merge_pairs_ind >>
 srw_tac [BAG_ss]
         [merge_pairs_def, pairing_heap_to_bag_def, pairing_heap_merge_bag]);
 
 val pairing_heap_merge_pairs_ok = Q.prove (
-`!leq hs.
-  WeakLinearOrder leq ∧ EVERY (pairing_heap_ok leq) hs
+`!get_key leq hs.
+  WeakLinearOrder leq ∧ EVERY (pairing_heap_ok get_key leq) hs
   ⇒ 
-  pairing_heap_ok leq (merge_pairs leq hs)`,
+  pairing_heap_ok get_key leq (merge_pairs get_key leq hs)`,
 recInduct merge_pairs_ind >>
 rw [merge_pairs_def, pairing_heap_ok_def, pairing_heap_merge_ok]);
 
 val pairing_heap_delete_min_thm = Q.store_thm ("pairing_heap_delete_min_thm",
-`!h leq. 
+`!h get_key leq. 
   WeakLinearOrder leq ∧
   (h ≠ Empty) ∧ 
-  pairing_heap_ok leq h 
+  pairing_heap_ok get_key leq h 
   ⇒ 
-  pairing_heap_ok leq (delete_min leq h) ∧
-  (pairing_heap_to_bag (delete_min leq h) = 
+  pairing_heap_ok get_key leq (delete_min get_key leq h) ∧
+  (pairing_heap_to_bag (delete_min get_key leq h) = 
    BAG_DIFF (pairing_heap_to_bag h) (EL_BAG (find_min h)))`,
 rw [] >>
 cases_on `h` >>
